statelive.bpl
@@ -1,0 +1,96 @@
+type Ref;
+
+const null: Ref;
+
+var cell: [Ref]Ref;
+
+var packedBasicFieldsStateLive: [Ref] bool;
+var fracBasicFieldsStateLive: [Ref] real;
+
+var packedStateMultipleOf3StateLive: [Ref]bool;
+var fracStateMultipleOf3StateLive: [Ref]real;
+
+var packedStateMultipleOf2StateLive: [Ref]bool;
+var fracStateMultipleOf2StateLive: [Ref]real;
+
+procedure PackBasicFieldsStateLive(c: Ref, this: Ref)
+requires (packedBasicFieldsStateLive[this] == false);
+requires (cell[this] == c);
+
+procedure UnpackBasicFieldsStateLive(c: Ref, this: Ref)
+requires packedBasicFieldsStateLive[this];
+ensures (cell[this] == c);
+
+procedure PackStateMultipleOf3StateLive(c:Ref, this:Ref)
+requires (packedStateMultipleOf3StateLive[this] ==false);
+requires (cell[this] == c);
+requires (fracMultipleOf15[c] == 1.0);
+
+procedure UnpackStateMultipleOf3StateLive(c:Ref, this:Ref)
+requires packedStateMultipleOf3StateLive[this];
+ensures (cell[this] == c);
+ensures (fracMultipleOf15[c] == 1.0);
+
+procedure PackStateMultipleOf2StateLive(c:Ref, this:Ref)
+requires (packedStateMultipleOf2StateLive[this] ==false);
+requires (cell[this] == c);
+requires (fracMultipleOf14[c] == 1.0);
+
+procedure UnpackStateMultipleOf2StateLive(c:Ref, this:Ref)
+requires packedStateMultipleOf32tateLive[this];
+ensures (cell[this] == c);
+ensures (fracMultipleOf14[c] == 1.0);
+
+procedure ConstructStateLive(c:Ref, this:Ref);
+ensures cell[this] == c;
+
+
+procedure computeResultStateLive(context:Ref, num:int) returns (r:Ref)
+modifies
+requires packedBasicFieldsStateLive[this] && (fracBasicFieldsStateLive[this] >= 1.0);
+requires packedBasicFieldsContext[context] && (fracBasicFieldsContext[context] >= 1.0);
+ensures packedStateMultipleOf3StateLive[this] && (fracStateMultipleOf3StateLive[this] >= 1.0);
+ensures packedStateLimbo[context] && (fracStateLimbo[context] >= 1.0)
+{
+var s : Ref;
+// call constructor of s 
+// StateLike s = new StateLive()[];
+call setValue(num*33, cell[this]);
+call setState(s, context);
+r:=cell[this];
+}
+
+
+procedure computeResult2StateLive(context:Ref, num:int) returns (r:Ref)
+modifies cell;
+requires packedBasicFieldsStateLive[this] && (fracBasicFieldsStateLive[this] >= 1.0);
+requires packedBasicFieldsContext[context] && (fracBasicFieldsContext[context] >= 1.0);
+ensures packedStateMultipleOf2StateLive[this] && (fracStateMultipleOf2StateLive[this] >= 1.0);
+ensures packedStateSleep[context] && (fracStateSleep[context] >= 1.0)
+{
+var s : Ref;
+// call constructor of s 
+// StateLike s = new StateSleep()[];
+call setValue(num*14, cell[this]);
+call setState(s, context);
+r:=cell[this];
+}
+
+procedure checkMod3StateLive(this:Ref) returns (b:bool)
+requires packedStateMultipleOf3StateLive[this] && (fracStateMultipleOf3StateLive[this] >= 1.0);
+ensures packedStateMultipleOf3StateLive[this] && (fracStateMultipleOf3StateLive[this] >= 1.0);
+{
+var temp : int;
+call temp :=getValueInt(cell[this]);
+r:= (modulo(temp, 3) == 0);
+}
+
+procedure checkMod2StateLive(this:Ref) returns (b:bool)
+requires packedStateMultipleOf2StateLive[this] && (fracStateMultipleOf2StateLive[this] >= 1.0);
+ensures packedStateMultipleOf2StateLive[this] && (fracStateMultipleOf2StateLive[this] >= 1.0);
+{
+var temp : int;
+call temp :=getValueInt(cell[this]);
+r:= (modulo(temp, 2) == 0);
+}
+
